\documentclass[psamsfonts]{amsart}
%
%-------Packages---------
%
\usepackage[h margin=1 in, v margin=1 in]{geometry}
\usepackage{amssymb,amsfonts}
\usepackage[all,arc]{xy}
\usepackage{enumerate}
\usepackage{mathrsfs}
\usepackage{amsthm}
\usepackage{mathpazo}
\usepackage{yfonts}
\usepackage{enumitem}
\usepackage{mathrsfs}
\usepackage{fourier-orns}
\usepackage[all]{xy}
\usepackage{hyperref}
\usepackage{cite}
\usepackage{url}
\usepackage{mathtools}
\usepackage{graphicx}
\usepackage{pdfsync}
\usepackage{mathdots}
%
\usepackage{tgpagella}
\usepackage[T1]{fontenc}
%
\usepackage{listings}
\usepackage{color}

\definecolor{dkgreen}{rgb}{0,0.6,0}
\definecolor{gray}{rgb}{0.5,0.5,0.5}
\definecolor{mauve}{rgb}{0.58,0,0.82}

\lstset{frame=tb,
  language=Matlab,
  aboveskip=3mm,
  belowskip=3mm,
  showstringspaces=false,
  columns=flexible,
  basicstyle={\small\ttfamily},
  numbers=none,
  numberstyle=\tiny\color{gray},
  keywordstyle=\color{blue},
  commentstyle=\color{dkgreen},
  stringstyle=\color{mauve},
  breaklines=true,
  breakatwhitespace=true,
  tabsize=3
  }
%
%--------Theorem Environments--------
%
\newtheorem{thm}{Theorem}[section]
\newtheorem*{thm*}{Theorem}
\newtheorem{cor}[thm]{Corollary}
\newtheorem{prop}[thm]{Proposition}
\newtheorem{lem}[thm]{Lemma}
\newtheorem*{lem*}{Lemma}
\newtheorem{conj}[thm]{Conjecture}
\newtheorem{quest}[thm]{Question}
%
\theoremstyle{definition}
\newtheorem{defn}[thm]{Definition}
\newtheorem*{defn*}{Definition}
\newtheorem{defns}[thm]{Definitions}
\newtheorem{con}[thm]{Construction}
\newtheorem{exmp}[thm]{Example}
\newtheorem{exmps}[thm]{Examples}
\newtheorem{notn}[thm]{Notation}
\newtheorem{notns}[thm]{Notations}
\newtheorem{addm}[thm]{Addendum}
\newtheorem{exer}[thm]{Exercise}
%
\theoremstyle{remark}
\newtheorem{rem}[thm]{Remark}
\newtheorem*{claim}{Claim}
\newtheorem*{aside*}{Aside}
\newtheorem*{rem*}{Remark}
\newtheorem*{hint*}{Hint}
\newtheorem*{note}{Note}
\newtheorem{rems}[thm]{Remarks}
\newtheorem{warn}[thm]{Warning}
\newtheorem{sch}[thm]{Scholium}
%
%--------Macros--------
\renewcommand{\qedsymbol}{$\blacksquare$}
\renewcommand{\hom}{\mathsf{Hom}}
\renewcommand{\emptyset}{\varnothing}
\newcommand{\R}{\mathbb{R}}
\newcommand{\ib}[1]{\textbf{\textit{#1}}}
\newcommand{\Q}{\mathbb{Q}}
\newcommand{\Z}{\mathbb{Z}}
\newcommand{\N}{\mathbb{N}}
\newcommand{\C}{\mathbb{C}}
\newcommand{\A}{\mathbb{A}}
\newcommand{\F}{\mathbb{F}}
\newcommand{\M}{\mathcal{M}}
\renewcommand{\S}{\mathbb{S}}
\newcommand{\V}{\vec{v}}
\newcommand{\RP}{\mathbb{RP}}
\newcommand{\CP}{\mathbb{CP}}
\newcommand{\B}{\mathcal{B}}
\newcommand{\GL}{\mathsf{GL}}
\newcommand{\SL}{\mathsf{SL}}
\newcommand{\SP}{\mathsf{SP}}
\newcommand{\SO}{\mathsf{SO}}
\newcommand{\SU}{\mathsf{SU}}
\newcommand{\gl}{\mathfrak{gl}}
\newcommand{\g}{\mathfrak{g}}
\newcommand{\inv}{^{-1}}
\newcommand{\bra}[2]{ \left[ #1, #2 \right] }
\newcommand{\ind}{\lambda \in \Lambda}
\newcommand{\set}[1]{\left\lbrace#1 \right\rbrace}
\newcommand{\imp}[2]{ \underline{ #1 \implies #2} }
\newcommand{\abs}[1]{\left\lvert#1\right\rvert}
\newcommand{\norm}[1]{\left\lVert#1\right\rVert}
\newcommand{\transv}{\mathrel{\text{\tpitchfork}}}
\newcommand{\enumbreak}{\ \\ \vspace{-\baselineskip}}
\let\oldexists\exists
\renewcommand\exists{\oldexists~}
\let\oldL\L
\renewcommand\L{\mathfrak{L}}
\makeatletter
\newcommand{\tpitchfork}{%
  \vbox{
    \baselineskip\z@skip
    \lineskip-.52ex
    \lineskiplimit\maxdimen
    \m@th
    \ialign{##\crcr\hidewidth\smash{$-$}\hidewidth\crcr$\pitchfork$\crcr}
  }%
}
\makeatother
\newcommand{\bd}{\partial}
\newcommand{\lang}{\begin{picture}(5,7)
\put(1.1,2.5){\rotatebox{45}{\line(1,0){6.0}}}
\put(1.1,2.5){\rotatebox{315}{\line(1,0){6.0}}}
\end{picture}}
\newcommand{\rang}{\begin{picture}(5,7)
\put(.1,2.5){\rotatebox{135}{\line(1,0){6.0}}}
\put(.1,2.5){\rotatebox{225}{\line(1,0){6.0}}}
\end{picture}}
\DeclareMathOperator{\id}{id}
\DeclareMathOperator{\im}{Im}
\DeclareMathOperator{\grap}{graph}
\DeclareMathOperator{\codim}{codim}
\DeclareMathOperator{\supp}{supp}
\DeclareMathOperator{\inter}{Int}
\DeclareMathOperator{\sign}{sign}
\DeclareMathOperator{\sgn}{sgn}
\DeclareMathOperator{\indx}{ind}
\DeclareMathOperator{\alt}{Alt}
\DeclareMathOperator{\Aut}{Aut}
\DeclareMathOperator{\trace}{trace}
\DeclareMathOperator{\ad}{ad}
\DeclareMathOperator{\End}{End}
\DeclareMathOperator{\Ad}{Ad}
\DeclareMathOperator{\Lie}{Lie}
\DeclareMathOperator{\spn}{span}
\DeclareMathOperator{\dv}{div}
\DeclareMathOperator{\grad}{grad}
\newcommand*\myhrulefill{%
   \leavevmode\leaders\hrule depth-2pt height 2.4pt\hfill\kern0pt}
\newcommand\niceending[1]{%
  \begin{center}%
    \LARGE \myhrulefill \hspace{0.2cm} #1 \hspace{0.2cm} \myhrulefill%
  \end{center}}
\newcommand*\sectionend{\niceending{\decofourleft\decofourright}}
\newcommand*\subsectionend{\niceending{\decosix}}
\def\upint{\mathchoice%
    {\mkern13mu\overline{\vphantom{\intop}\mkern7mu}\mkern-20mu}%
    {\mkern7mu\overline{\vphantom{\intop}\mkern7mu}\mkern-14mu}%
    {\mkern7mu\overline{\vphantom{\intop}\mkern7mu}\mkern-14mu}%
    {\mkern7mu\overline{\vphantom{\intop}\mkern7mu}\mkern-14mu}%
  \int}
\def\lowint{\mkern3mu\underline{\vphantom{\intop}\mkern7mu}\mkern-10mu\int}
%
%--------Hypersetup--------
%
\hypersetup{
    colorlinks,
    citecolor=black,
    filecolor=black,
    linkcolor=blue,
    urlcolor=black
}
%
%--------Solution--------
%
\newenvironment{solution}
  {\begin{proof}[Solution]}
  {\end{proof}}
%
%--------Graphics--------
%
%\graphicspath{ {images/} }

\begin{document}
\author{Jeffrey Jiang}
\title{The Laplace-de Rham Operator on a Riemannian Manifold}
\maketitle
%
\setcounter{section}{1}
%
In $\R^2$, we know about the standard Laplace operator on $C^\infty(\R^2)$
$$\Delta = \frac{\partial^2}{\partial x^2} + \frac{\partial^2 }{\partial y^2}$$
In a more general setting, let $(M,g)$ be a Riemannian manifold. We can define an analogous operator
$$\Delta = \dv(\grad f) $$
In local coordinates $(x^i)$, we have that  for $f \in C^\infty(M)$  and $X \in \mathfrak{X}(M)$
\begin{align*}
\grad f &= g^{ij}\frac{\partial f}{\partial x^i}\frac{\partial }{\partial x^j} \\[6pt]
\dv X &= \frac{1}{\sqrt[â€¢]{\det  g_{ij}}} \frac{\partial}{\partial x^i}\left((X^i \sqrt{\det g_{ij}}\right)
\end{align*}
Where $g_{ij}$ is the symmetric matrix given by $g_{ij} = \langle \partial_i ,\partial_j\rangle$ and $g^{ij}$ is the inverse of $g_{ij}$. This gives the coordinate formula for 
$$\Delta f = \frac{1}{\sqrt{\det g_{ij}}} \frac{\partial}{\partial x^i}\left( g^{ij} \sqrt{\det g_{ij}}\frac{\partial f}{\partial x^j} \right)$$
Which using the standard metric $g_{ij} = \delta_{ij}$ on $\R^2$ recovers the standard Laplacian. However, we want to generalize $\Delta$ to arbitrary differential forms, which requires us to construct a  bit of machinery.

To do this, we first note that the metric $g$ determines an inner product on each tangent space $T_pM$ where $\langle v, w \rangle = g_p(v,w)$. From this, we can construct an inner product on the alternating tensors $\Lambda^k(T_pM)$, which will give us a smoothly varying inner product on $\Omega^K(M)$. To  do this, we will use the fact that $g$ determines a bundle isomorphism $TM \to  T^*M$ via the mapping $(x,v) \mapsto (x, \langle v, \cdot \rangle )$.
%
\begin{prop}
For a Riemannian manifold $(M,g)$,  there is a unique inner product on each $\Lambda^k(T_pM)$ characterized by the formula
$$\langle \omega^1 \wedge \ldots \wedge w^k, \eta^1 \wedge \ldots \wedge \eta^k = \det\left( \langle (\omega^i)^\sharp, (\eta^j)^\sharp \right) \rangle $$
Where $\sharp$ is the index raising operator $\omega_i dx^i \mapsto g^{ij}\omega_j\frac{\partial}{\partial x^i}$.
\end{prop}
%
\begin{proof}
We define the inner product locally in terms of an orthonomal frame $E_i$, and show that it is independent of the choice of frame. Let $\varepsilon^i$  denote the coframe to  $E_i$. We first claim that the set of $\varepsilon^I$ where $I$  is a strictly increasing multi-index of length $k$ form an orthonormal basis. To see this, we compute 
\begin{align*}
\langle \varepsilon^I, \varepsilon^J \rangle &= \det\left( E_{i_k}, E_{j_\ell} \right) 
\end{align*}
We note that this is $1$ if and only if $I = J$, since then the matrix we are taking the determinant of is $\id_{\R^k}$, otherwise, $I$  contains some $i_k$ not in  $J$, which implies the $k^{th}$ row of the matrix is $0$, so the determinant is $0$. This then defines an inner product by extending linearly to arbitrary $k$-forms.

To show that this is independent of our choice of frame, let  $B_i$ be another orthonormal frame with coframe $\beta^i$. Then we know that $B_i = A^j_iE_j$ with smooth functions $A^i_j$ forming an orthogonal matrix every point. We then compute
\begin{align*}
\langle \beta^I, \beta^J \rangle &= \det \langle B_{i_k}, B_{j_\ell} \rangle \\
&= \det\langle A^j_{i_k}E_j, A^p_{j_\ell}E_p \rangle \\
\end{align*}
Noting that $A^j_{i_k}E_j$ is just the $i_k^{th}$ column of the matrix $A$, we have that this is equal to $\det \langle A_{i_k}, A_{j_\ell} \rangle$. Again, if $I = J$, this is just the identity matrix, but if $I \neq J$, there will be a row of zeroes in the matrix $\langle A_{i_k}, A_{j_\ell}$, so the determinant will be $0$. This shows that $\langle \cdot, \cdot \rangle$  is uniquely characterized. 
\end{proof}
\begin{rem*}
One observation is that the Riemannian volume form $dV_g$  is the unique $n$-form on $M$ with norm $1$.
\end{rem*}
We can then use this inner product to produce an important operator. Recall that given a function $f \in C^\infty(M)$, we can define the integral of $f$ over $M$ by integrating the $n$-form $fdV_g$, which is a bundle homomorphism $\Omega^0(M) \to \Omega^n(M)$. We can generalize this to arbitrary $k$ forms.
\begin{prop}
For every $k \in \set{0, \ldots  n}$, there exists a unique bundle homomorphism
$$\star: \Omega^{k}(M) \to \Omega^{n-k}(M)$$
called the \ib{Hodge star operator} such that for any $\omega, \eta  \in \Omega^k(M)$, we have that $\omega \wedge \star\eta = \langle \omega, \eta \rangle dV_g$ where $dV_g$ is the Riemannian volume form. The $n-k$-form $\star \omega$ is often referred to as the \ib{Hodge dual} to $\omega$
\end{prop}
\begin{proof}
We first prove uniqueness. Let $\varepsilon^i$  be the coframe to an orthonomal basis $E_i$. Then for and increasing index set $I$ of length $k$, we have that $\star$ must satisify 
$$\varepsilon \wedge \star \varepsilon^I = dV_g$$
Therefore, we must have that $\star \varepsilon^I = \pm \varepsilon^J$, where $I \cup J = \set{1, \ldots n}$ and $J$ is an increasing index and the sign are chosen such that when we permute $I$ and $J$ to be in increasing order, the sign chosen for $\star \varepsilon^I$ cancel the ones that come from the permutation, since otherwise, $\varepsilon \wedge \star \varepsilon^I = 0$. This uniquely characterizes $\star$ on a basis, so it uniquely extends linearly to $\Omega^k(M)$.
\end{proof}

One observation we make is that $\star\star \varepsilon^I = (-1)^{k(n-k)}\varepsilon^I$ ,which can be verified by shuffling the wedge products and carefully tracking signs. This extends to all $k$-forms, so $\star \star\omega = (-1)^{k(n-k)}\omega$. Another observation is that this determines a bundle \emph{isomorphism} $\Omega^k(M) \to \Omega^{n-k}(M)$, since it maps an orthonormal basis to an orthonormal basis.
\begin{exmp}
In $\R^n$ with the standard coordinates $x^i$  and the standard metric tensor  $g_{ij} = \delta_{ij}$, we have that the $dx^i$ form an global orthonormal frame for $\R^n$. Given any $dx^i$, we have that 
$$\star dx^i =  (-1)^{i-1} dx^1 \wedge \ldots \wedge \hat{dx^i} \wedge \ldots \wedge dx^n $$
Where $\hat{dx^i}$ indicates that $dx^i$ is missing  from the wedge product. The sign comes from the fact that 
$$dx^i \wedge dx^1 \wedge \ldots \wedge \hat{dx^i} \wedge \ldots \wedge dx^n = (-1)^{i-1} dx^1\wedge \ldots \wedge dx^n$$
\end{exmp}
%
\begin{exmp}
For $\R^5$,  consider $\star\star dx^1 \wedge dx^3$. We first compute
$$\star dx^1 \wedge dx^3 = -dx^2 \wedge dx^4 \wedge dx^5 $$
$$\star\star dx^1\wedge dx^3 = \star -dx^2 \wedge dx^4 \wedge dx^5 = dx^1 \wedge d^3$$
\end{exmp}
%
Finally, we can use the Hodge star to define yet another operator
\begin{defn}
Let $(M,g)$ be a compact oriented Riemannian manifold. Then the \ib{codifferential} $\delta$ (also denoted in the literature by $d^*$) is a map
\begin{align*}
\delta: \Omega^k(M) &\to \Omega^{k-1}(M) \\
\delta \omega &= (-1)^{n(k+1)+1}\star d \star \omega
\end{align*}
Where $\delta$ is  defined on $\Omega^0(M) = C^\infty(M)$ by  $\delta f = 0$ for all smooth functions $f$.
\end{defn}
%
\begin{prop}
The codifferential $\delta$ on  a Riemannian manifold $(M,g)$ without boundary satisfies the following properties:
\begin{enumerate}
\item $\delta^2 = 0$ 
\item For $\omega,\eta \in \Omega^k(M)$, let 
$$(\omega, \eta) = \int_M \langle \omega, \eta \rangle ~dV_g$$
Then for $\omega \in \Omega^k(M)$ and $\eta \in \Omega^{k-1}(M)$, we have that 
$$(\delta \omega, \eta) = (\omega, d\eta) $$
where $d$ is the exterior derivative. In this way, we see that $\delta$  is the \ib{adjoint} of $d$ with respect to the inner product, justifying the name \ib{codifferential}.
\end{enumerate}
\end{prop}

\begin{proof}
\begin{enumerate}
\item We have that
\begin{align*}
\delta^2 &= (-1)^{n(k+1)+1} \delta \star d \star \\
&= (-1)^{n(k+1) + 1}(-1)^{nk + 1} \star d \star \star d \star
\end{align*}
We note that $\star\star = (-1)^{k(n-k)}\id_{\Omega^k(M)}$, so this simplifies to
$$(-1)^p \star d d \star = 0 $$
Since $d^2 = 0$.
\item We first verify that $(\cdot, \cdot)$ determines  an inner product. We note that it is symmetric since $\langle  \cdot, \cdot \rangle$ is symmetric, and it is also bilinear since integration is linear and $\langle \cdot, \cdot \rangle$ is as well. All that remains is to show that it is positive definite. We note that it is positive since $\langle \omega, \omega \rangle$ is positive for all $\omega$, so 
$$\int_M \langle\omega,\omega\rangle dV_g > 0$$
. In addition, we have that $\langle \omega, \omega \rangle = 0$ if and only if $\omega = 0$, and $\int_M fdV_g = 0$ if and only  if $f = 0$. Therefore, $(\cdot,\cdot)$ is positive definite, so it defines an inner product on $\Omega^k(M)$.

We note that by how we've define the $\star$ operator, the inner product is given  by the equivalent definition for $\xi, \alpha \in \Omega^k(M)$
$$(\xi, \alpha) = \int_M \xi \wedge \star \alpha $$
Therefore, we wish to  prove the equivalent statement that for $\omega \in \Omega^k(M)$ and $\eta
\in \Omega^{k-1}(M)$
$$\int_M  \delta\omega \wedge \star\eta = \int_M \omega \wedge \star d\eta $$
Then using symmetry of the inner product, this is equivalent to the statement
$$\int_M \eta \wedge \star\delta\omega = \int_M d\eta \wedge \star\omega $$
We then compute
\begin{align*}
d\eta \wedge \star\omega - \eta \wedge \star\delta\omega &= d\eta \wedge\star\omega - (-1)^{n(k+1)+1}\eta \wedge \star\star d\star\omega \\
&= d\eta \wedge \star\omega - (-1)^{n(k+1)+1}(-1)^{(n-k+1)(n-(n-k+1))}\eta \wedge d\star\omega \\
&= d\eta \wedge \star\omega + (-1)^{-k^2 + 1}  \eta \wedge d\star\omega \\
&= d\eta \wedge  \star\omega + (-1)^{k-1}\eta\wedge d\star\omega \\
&= d(\eta \wedge \star\omega)
\end{align*}
Where we use the fact that $-k^2  + 1$ has the opposite parity of $k$, and that $d$ is an antiderivation on $\Omega(M)$
Therefore, we have by Stokes' Theorem
$$\int_M d\eta \wedge \star\omega - \eta \wedge \star d\omega = \int_M d(\eta \wedge\star\omega) = \int_{\partial M} \eta \wedge  \star\omega = 0 $$
Which gives us that 
$$ (\delta\omega, \eta)= (\omega,d\eta)$$
\end{enumerate}
\end{proof}
Finally,  we have the necessary tools to define the fabled \ib{Laplace-de Rham Operator} (Also known as the  \ib{Laplace-Beltrami Operator}.
\begin{defn}
On a oriented compact Riemannian manifold $(M,g)$, define the \ib{Laplace-de Rham Operator}, denoted $\Delta$, as  the family of maps $\Omega^k(M) \to \Omega^k(M)$ such that 
$$\Delta = \delta d + d\delta $$
A $k$-form $\omega$ satsifying $\Delta\omega = 0$ is called \ib{harmonic}.
\end{defn}

\begin{prop}
The Laplace-de Rahm operator agrees with (up to sign) to the Laplacian on $C^\infty(M)$
\end{prop}
%
\begin{proof}
We have that for $f \in C^\infty(M)$ (letting $\Delta$ denote the Laplace-de Rham operator)
$$\Delta f  = d\delta f + \delta d f = \delta df$$
Since we defined $\delta$ to be $0$ on $\Omega^0(M) = C^\infty(M)$.
We then have that $\delta df = -\star d\star df$. We first compute $\star df$, which is the $n-1$-form satisfying 
$$df \wedge \star df = \langle df, df \rangle ~dV_g $$. Noting that $df^\sharp = \grad f$, we compute
\begin{align*}
\langle \grad f, \grad f\rangle ~dV_g &= \frac{\partial f}{\partial x^i} dx^i \left( g^{jk}\frac{\partial f}{\partial j}\frac{\partial}{\partial x^k} \right)~dV_g \\
&= g^{ij}\frac{\partial  f}{\partial x^i}\frac{\partial f}{\partial x^j} ~dV_g \\
&= \sqrt{\det g}\left( g^{ij}\frac{\partial  f}{\partial x^i}\frac{\partial f}{\partial x^j} dx^1 \right)\wedge \ldots \wedge dx^n
\end{align*}
Therefore, we conclude that
$$\star df = (-1)^{i-1}\sqrt{\det g} \left(g^{ij}\frac{\partial f}{\partial x^j} \right)dx^1 \wedge \ldots \hat{dx^i} \wedge \ldots \wedge dx^n $$
\end{proof}
We then compute $d\star df$ to be 
\begin{align*}
d\star df &= (-1)^{i-1} \frac{\partial}{\partial x^k}\left( g^{ij}\sqrt{\det g}\frac{\partial f}{\partial x^j} \right) dx^k \wedge dx^1 \wedge \ldots \wedge \hat{dx^i} \wedge \ldots \wedge dx^n \\
&= \frac{\partial}{\partial x^i}\left( g^{ij}\sqrt{\det g}\frac{\partial f}{\partial x^j} \right) dx^1 \wedge \ldots \wedge dx^n \\
&= \frac{1}{\sqrt{\det g}} \frac{\partial}{\partial x^i}\left( g^{ij}\sqrt{\det g}\frac{\partial f}{\partial x^j} \right) dV_g
\end{align*}

We then have that $\star d\star df$ must satsify $d\star f \wedge \star d\star df = \langle d\star f, d\star f \rangle~dV_g$. We then compute
\begin{align*}
\biggl\langle \frac{1}{\sqrt{\det g}} \frac{\partial}{\partial x^i}\left( g^{ij}\sqrt{\det g}\frac{\partial f}{\partial x^j} \right) dV_g, \frac{1}{\sqrt{\det g}} \frac{\partial}{\partial x^k}\left( g^{k\ell}\sqrt{\det g}\frac{\partial f}{\partial x^\ell} \right)~dV_g\biggr\rangle~dV_g  \\
= \frac{1}{\det g}\frac{1}{\sqrt{\det g}} \frac{\partial}{\partial x^i}\left( g^{ij}\sqrt{\det g}\frac{\partial f}{\partial x^j} \right)    \frac{1}{\sqrt{\det g}} \frac{\partial}{\partial x^k}\left( g^{k\ell}\sqrt{\det g}\frac{\partial f}{\partial x^k} \right) ~dV_g
\end{align*}
Where we use the fact that $\langle dV_g, dV_g \rangle = 1$. Therefore, we conclude that 
$$\delta df = -\star d\star f = -\frac{1}{\sqrt{\det g}} \frac{\partial}{\partial x^i}\left( g^{ij}\sqrt{\det g}\frac{\partial f}{\partial x^j} \right) $$
Due to our choice of sign convention, this is unfortunately the negative of the the original Laplacian we had. Some sign conventions define $\Delta f = -\dv(\grad f)$ for this reason.

%
\end{document}